Zippy/Zippy/Goal_Pos_Updates/Zippy_Goal_Pos_Updates.thy
@@ -13,8 +13,8 @@ ML_file\<open>zippy_goals_pos_mixin.ML\<close>
 
 (*ground polymorphic types since only ground types can be stored in the generic context.*)
 setup\<open>Context.theory_map ML_Gen.ground_zipper_types\<close>
-ML_file\<open>zippy_init_goal_clusters_mixin_base.ML\<close>
-ML_file\<open>zippy_init_goal_clusters_mixin.ML\<close>
+ML_file\<open>zippy_update_goal_cluster_mixin_base.ML\<close>
+ML_file\<open>zippy_update_goal_cluster_mixin.ML\<close>
 (*reset grounding*)
 setup\<open>Context.theory_map ML_Gen.reset_zipper_types\<close>
 
