Zippy/Zippy/Lists/Zippy_Lists_Base.thy
@@ -3,10 +3,7 @@ theory Zippy_Lists_Base
   imports
     ML_Zipper_Instances
     Zippy_Enums
-    Zippy_Loggers
     Zippy_Nodes
-    Zippy_Shows
-    Zippy_States
 begin
 
 ML_file\<open>zippy_lists_base.ML\<close>
